ML. It's a mystery to me.

thy/OpenFlow/IpRoute_Parser.ml
@@ -1,0 +1,75 @@
+local
+  fun define_const (t: term) (name: binding) (lthy: local_theory) : local_theory = let
+        val _ = writeln ("Defining constant `"^Binding.name_of name^"' ("^Binding.name_of name^"_def')");
+        val ((_, (_, thm)), lthy) = Local_Theory.define ((name, NoSyn), ((Binding.empty, []), t)) lthy;
+        val (_, lthy) = Local_Theory.note ((Binding.suffix_name "_def" name, @{attributes [code]}), [thm]) lthy;
+       in
+         lthy
+  end
+  fun load_file (thy: theory) (path: string list) =
+      let val p =  File.full_path (Resources.master_directory thy) (Path.make path); in
+      let val _ = "loading file "^File.platform_path p |> writeln; in
+        if not (File.exists p) orelse (File.is_dir p) then raise Fail "File not found" else File.read_lines p
+   end end;
+
+  (* and now, some code duplication with the IPtables parser\<dots> *)
+  fun extract_int ss = case ss |> implode |> Int.fromString of SOME i => i
+                                                             | NONE => raise Fail "unparsable int";
+
+  fun is_iface_char x = Symbol.is_ascii x andalso
+      (Symbol.is_ascii_letter x orelse Symbol.is_ascii_digit x orelse x = "+" orelse x = "*" orelse x = ".")
+  fun mk_nat maxval i = if i < 0 orelse i > maxval
+            then
+              raise Fail("nat ("^Int.toString i^") must be between 0 and "^Int.toString maxval)
+            else (HOLogic.mk_number HOLogic.natT i);
+  val mk_nat255 = mk_nat 255;
+
+  fun mk_quadrupel (((a,b),c),d) = HOLogic.mk_prod
+               (mk_nat255 a, HOLogic.mk_prod (mk_nat255 b, HOLogic.mk_prod (mk_nat255 c, mk_nat255 d)));
+  fun ipprefix_to_hol (ip,len) = @{const PrefixMatch} $ (@{const ipv4addr_of_dotdecimal} $ (mk_quadrupel ip)) $ mk_nat 32 len;
+
+  val parser_ip = (Scan.many1 Symbol.is_ascii_digit >> extract_int) --| ($$ ".") --
+                  (Scan.many1 Symbol.is_ascii_digit >> extract_int) --| ($$ ".") --
+                  (Scan.many1 Symbol.is_ascii_digit >> extract_int) --| ($$ ".") --
+                  (Scan.many1 Symbol.is_ascii_digit >> extract_int);
+  
+  val parser_ip_cidr = parser_ip --| ($$ "/") -- (Scan.many1 Symbol.is_ascii_digit >> extract_int) >> ipprefix_to_hol;
+  
+  val parser_interface = Scan.many1 is_iface_char >> (implode #> (fn x => HOLogic.mk_string x));
+  (* end dup *)
+  
+  val parser_subnet = parser_ip_cidr ||
+    (parser_ip >> (fn ip => ipprefix_to_hol (ip,32))) ||
+    (Scan.this_string "default" >> K @{term "PrefixMatch 0 0"})
+  val parser_whitespace = Scan.many1 (fn x => x = " ");
+  
+  val parser_via = (Scan.this_string "via" -- parser_whitespace |-- parser_ip) >> mk_quadrupel
+  val parser_dev = (Scan.this_string "dev" -- parser_whitespace |-- parser_interface)
+  val parser_metric = (Scan.this_string "metric" -- parser_whitespace |-- Scan.many1 Symbol.is_ascii_digit >> extract_int)
+  (* these are going to be ignored anyway\<dots>(?) *)
+  val parser_scope = (Scan.this_string "scope" -- parser_whitespace |-- (
+    Scan.this_string "host" || Scan.this_string "host" || Scan.this_string "host" || (Scan.many1 Symbol.is_ascii_digit >> implode)))
+  val parser_proto = (Scan.this_string "proto" -- parser_whitespace |-- (
+    Scan.this_string "kernel" || Scan.this_string "boot" || Scan.this_string "static" || (Scan.many1 Symbol.is_ascii_digit >> implode)))
+  val parser_src = (Scan.this_string "src" -- parser_whitespace |-- parser_ip) >> mk_quadrupel
+
+  fun parse_loop r =
+    
+  
+  fun parser tp =
+    (parser_subnet >> (fn x => @{const empty_rr_hlp} $ x)) tp
+in
+	fun register_ip_route (name,path) (lthy: local_theory) =
+	let
+	  val fcontent = load_file @{theory} [path]
+	  (*val _ = map writeln fcontent*)
+	  (*val _ = (Pretty.writeln o Syntax.pretty_term @{context} o fst o parser_subnet o Symbol.explode) "10.13.37.0/24 via 255.255.255.0 dev tun0"*)
+	  val _ = (Pretty.writeln o Syntax.pretty_term @{context} o snd o fst o
+	    (parser_subnet --| parser_whitespace -- parser_via) o Symbol.explode) "10.13.37.0/24 via 255.255.255.0 dev tun0"
+	  (*val _ = (Pretty.writeln o Syntax.pretty_term @{context} o fst o parser_subnet o Symbol.explode) "10.13.37.0/24 via 255.255.255.0 dev tun0"*)
+	  val r = map (parser o Symbol.explode #> fst) fcontent
+	  (*val _ = map (Pretty.writeln o (Syntax.pretty_term @{context})) r*) 
+	in
+	  define_const (HOLogic.mk_list @{typ "routing_rule"} r) name lthy
+	end
+end
